theories/coneris/examples/parallel_add.v
@@ -22,7 +22,7 @@ Section lemmas.
     own γ (●E b) -∗ own γ (◯E c) -∗ ⌜ b = c ⌝.
   Proof.
     iIntros "Hγ● Hγ◯".
-    by iCombine "Hγ● Hγ◯" gives %<-%excl_auth_agree_L.
+    by iCombine "Hγ● Hγ◯" gives %->%excl_auth_agree_L.
   Qed.
 
   Lemma ghost_var_update γ b' b c :
